refocusing_lang.v
@@ -2,41 +2,127 @@ Require Export Util.
 Require Import Program.
 
 
+
+(* Signature for languages with reduction semantics and multiple kinds of contextes. *)
+
 Module Type RED_LANG.
 
-  (** The languages of terms, values, redex, and context, the empty context is also needed. *)
-  Parameters term ckind elem_context : Set. 
-  Parameters value redex : ckind -> Set.
-  Parameter  ckind_trans : ckind -> elem_context -> ckind.
-  Notation "k +> ec" := (ckind_trans k ec) (at level 50, left associativity).
-  Parameter  init_ckind : ckind.
-  Parameter  dead_ckind : ckind -> Prop.
 
-  Axiom ckind_death_propagation : 
+  (* Note: (This describes only the simples use case.)
+     The only grammar mentioned in this formalization is a grammar of contexts,
+     thus any reference to a grammar means the grammar of contexts of the formalized
+     language.
+
+     In this formalisation we do not have a represenation for usual terminal 
+     symbols in the grammar. Instead, we take whole right sides of productions that 
+     contain non-terminals with non-terminals replaced by holes as terminals. Such 
+     right sides are called elementary contexts.
+
+     E.g., if k1, k2 are non-terminals and a, b, c are terminals, then the production 
+     k1 -> a b k2 c  may be represented as  k1 -> (a b [] c) k2  , where  a b [] c  
+     is an elementary context.
+
+     Now, if we require all right sides that do not contain non-terminals to be 
+     holes and existance of a production  k -> []  for any k, we can represent whole
+     grammar only in terms of elementary contexts and non-terminals.
+
+     We will call a hole generated from a symbol k >a hole of kind k< .
+
+     Because each production has at most one non-terminal symbol this procedure 
+     simplifies grammars of contexts to regular grammars on words. Let us call these 
+     grammars >linearized grammars< .
+
+     The requirement of productions  k -> []  does not break generality in our case,
+     because we will later fix redexes that can occur in each kind of holes. So
+     if we do not have a production  k -> []  in the original grammar, then we can 
+     equvalently fix redexes for k as an empty set. *)
+
+
+
+  (* Preconditions: To instaniate this module you need to linearize and determinize 
+     the grammar of contextes of your language. If the result grammar is not total, 
+     you need to include a sink non-terminal and totalize the grammar. *)
+
+
+
+  Parameters term  elem_context : Set.
+  Parameter  ckind : Set. (* kinds of contexts, that is, non-terminal symbols in 
+                             the grammar *)
+
+
+  Parameter  init_ckind : ckind. (* start symbol in the grammar *)
+  Parameter  dead_ckind : ckind -> Prop. (* set of sink symbols *)
+
+
+  (* ckind_trans - function that determinates the productions in the grammar, or 
+                   in other words, a transition function of a finit automaton 
+                   representing the grammar. *)
+  Parameter  ckind_trans : ckind -> elem_context -> ckind.
+  Infix "+>" := ckind_trans (at level 50, left associativity).
+
+
+  Axiom death_propagation : 
       forall k, dead_ckind k -> forall ec, dead_ckind (k+>ec).
 
 
-  Inductive context : ckind -> ckind -> Set :=
-  | empty : forall {k}, context k k
-  | ccons : forall (ec : elem_context) {k1 k2}, context k1 k2 -> context k1 (k2+>ec).
-  Notation "[_]" := empty.
-  Infix "=:" := ccons (at level 60, right associativity).
 
-  (** The main functions of reduction semantics, defining plugging terms into contexts and
-      composing contexts, effectively defining reduction semantics, and some properties. *)
-  Fixpoint compose {k1 k2} (c0 : context k1 k2) {k3} (c1 : context k3 k1) : context k3 k2 := 
-      match c0 in context k1' k2' return context k3 k1' -> context k3 k2' with
-      | [_]     => fun c1' => c1'
-      | ec=:c0' => fun c1' => ec =: compose c0' c1'
-      end c1.
-  Infix "~+" := compose (at level 60, right associativity).
+  (* context k1 k2 - contexts of kind k1 (derivated from k1) with the hole of kind k2. 
+                     Contexts are represented by reversed derivations from the grammar.
+                     E.g., if a context is derivated by a sequence of productions
+                     k1 -> ec1 k2, k2 -> ec2 k3, k3 -> ec3 k4, k4 -> [], then it is 
+                     represented by the list  (ec3, k4)=:(ec2, k3)=:(ec1, k2)  and the
+                     type of it is  context k1 k4  .
+                     The second elements in the pairs are implicite. *)
+  Inductive context (k1 : ckind) : ckind -> Set :=
+  | empty : context k1 k1
+  | ccons : forall (ec : elem_context) {k2}, context k1 k2 -> context k1 (k2+>ec).
+  Arguments empty {k1}. Arguments ccons {k1} _ {k2} _.
+  Notation "[.]"      := empty.
+  Notation "[.]( k )" := (@empty k).
+  Infix    "=:"       := ccons (at level 60, right associativity).
+
+  (* Note: Contexts are reversed, because during evaluation by refocusing we always 
+     access the elem. context nearest to the hole of a context. *)
+
+  (* Definition: The hole of a context is >dead< if its kind is a sink symbol. *)
+  (* Definition: A context is >proper< if its hole is not dead. 
+     (Context with dead holes are contexts that cannot be generated in the orginal
+     grammar.) *)
 
 
-  Axiom proper_death : forall k1, dead_ckind k1 -> 
-                           ~ exists k2 (c : context k1 k2) (r : redex k2), True.
+
+  (* Plugging is standard. You need to provide only plugging function for elem.
+     contexts. *)
+
+  Parameter elem_plug : term -> elem_context -> term.
+  Notation "ec :[ t ]" := (elem_plug t ec) (at level 0, t at level 99).
+
+  Fixpoint plug (t : term) {k1 k2} (c : context k1 k2) : term :=
+      match c with
+      | [.]    => t 
+      | ec=:c' => plug ec:[t] c'
+      end.
+  Notation "c [ t ]" := (plug t c) (at level 0, t at level 99).
+
+  (* The following axiom somehow relates our representation of contexts to real
+     contexts, but generally we can instantiate the module with elem. contexts
+     that do not represent real elem. contexts. *)
+  Axiom elem_plug_injective1 : forall ec {t0 t1},
+      ec:[t0] = ec:[t1] -> t0 = t1.
 
 
-  (** The values and redexes are sublanguages of terms *)
+  Definition immediate_ec ec t := exists t', ec:[t'] = t.
+
+
+
+  (* redex k - representations of redexes that may occur in a hole of the kind k. 
+     value k (where k is not a sink)
+             - (almost) normal forms of kind k, that is, representations of terms
+               that cannot be decomposed to a context k k' and a redex k'.  value k
+               where k is a sink may be anything. *)
+  Parameters value redex : ckind -> Set.
+
+
   Parameter value_to_term : forall {k}, value k -> term.
   Coercion  value_to_term : value >-> term.
   Parameter redex_to_term : forall {k}, redex k -> term.
@@ -48,41 +134,28 @@ Module Type RED_LANG.
       forall {k} (r r' : redex k), redex_to_term r = redex_to_term r' -> r = r'.
 
 
-  Parameter atom_plug : term -> elem_context -> term.
-  Notation "ec :[ t ]" := (atom_plug t ec) (at level 0, t at level 99).
-
-  Axiom atom_plug_injective1 : forall ec {t0 t1},
-      ec:[t0] = ec:[t1] -> t0 = t1.
-
-  Fixpoint plug (t : term) {k1 k2} (c : context k1 k2) : term :=
-      match c with
-      | [_]    => t 
-      | ec=:c' => plug ec:[t] c'
-      end.
-  Notation "c [ t ]" := (plug t c) (at level 0, t at level 99).
-
-  Definition strict_ec ec t := exists t', ec:[t'] = t.
+  (* A key property of sink non-terminals: *)
+  Axiom proper_death : forall k1, dead_ckind k1 -> 
+                           ~ exists k2 (c : context k1 k2) (r : redex k2), True.
 
 
-  (** The other main function of reduction semantics -- contraction of a redex into a term *)
-  Parameter contract : forall {k}, redex k -> option term.
+  (* Definition: A decomposition c[t] is empty if c is empty. *)
+  (* Definition: A decomposition c[t] is proper if c is proper. *)
 
-
-(*  Definition transitable_from k ec := ~ dead_ckind (k+>ec).
-  Definition ec_siblings ec0 ec1 := 
-      exists t0 t1, atom_plug t0 ec0 = atom_plug t1 ec1.*)
-
+  (* only_empty t k   - the term t has only empty or improper decompositions from 
+                        the non-terminal k.
+     only_trivial t k - each proper decomposition of the term t from the symbol k is 
+                        either empty or the component term is a value. *)
   Definition only_empty t k :=
       forall t' {k'} (c : context k k'), c[t'] = t -> ~ dead_ckind k' -> 
           k = k' /\ c ~= @empty k.
-
   Definition only_trivial t k :=
       forall t' {k'} (c : context k k'), c[t'] = t -> ~ dead_ckind k' -> 
           k = k' /\ c ~= @empty k \/ exists (v : value k'), t' = v.
 
 
+  (* Axioms of normal forms: *)
   Axiom value_trivial : forall {k} (v : value k), only_trivial v k.
-  Axiom redex_trivial : forall {k} (r : redex k), only_trivial r k.
   Axiom value_redex   : forall {k} (v : value k) (r : redex k), 
                             value_to_term v <> redex_to_term r.
   Axiom trivial_val_red : 
@@ -90,39 +163,69 @@ Module Type RED_LANG.
          (exists (v : value k), t = v) \/ (exists (r : redex k), t = r).
 
 
-  (** Datatype of decompositions -- either a value or a redex in a context 
-      (analogous to the decompose lemma) *)
-  Inductive decomp k : Set :=
-  | d_val : value k -> decomp k
-  | d_red : forall {k'}, redex k' -> context k k' -> decomp k.
 
+  (* Reduction of a redex (which may get stuck): *)
+  Parameter contract : forall {k}, redex k -> option term.
+
+
+
+  (* decomp k  - decomposition of a term t from the symbol k to a redex.
+     d_red r c - t = c[r].
+     d_val v   - t has no redexes and so it is a value, t = v. *)
+  Inductive decomp k : Set :=
+  | d_red : forall {k'}, redex k' -> context k k' -> decomp k
+  | d_val : value k -> decomp k.
   Arguments d_val {k} _. Arguments d_red {k} {k'} _ _.
 
   Definition decomp_to_term {k} (d : decomp k) :=
       match d with
-      | d_val v      => value_to_term v
-      | d_red _ r c0 => c0[r]
+      | d_val v     => value_to_term v
+      | d_red _ r c => c[r]
       end.
   Coercion decomp_to_term : decomp >-> term.
 
 
-  Inductive interm_dec k : Set :=
-  | in_red  : redex k -> interm_dec k
-  | in_val  : value k -> interm_dec k
-  | in_term : term -> elem_context -> interm_dec k
-  | in_dead : interm_dec k.
 
-  Arguments in_red {k} _. Arguments in_val {k} _. Arguments in_term {k} _ _.
+  (* Standard contexts composition: *)
+  Fixpoint compose {k1 k2} (c0 : context k1 k2) 
+                      {k3} (c1 : context k3 k1) : context k3 k2 := 
+      match c0 in context _ k2' return context k3 k2' with
+      | [.]     => c1
+      | ec=:c0' => ec =: compose c0' c1
+      end.
+  Infix "~+" := compose (at level 60, right associativity).
 
 End RED_LANG.
 
 
 
-Module Type RED_REF_LANG.
+Module Type DEC_STEP (R : RED_LANG).
 
-  Declare Module R : RED_LANG.
   Import R.
 
+
+  (* interm_dec k - result of functions performing one step of decomposition of 
+                    a term t from the symbol k to a redex.
+     in_red r      - t is a redex, t = r.
+     in_term t' ec - t = ec[t'] and to find a redex we are going to check t'.
+     in_val v      - there is no redexes in t, t = v.
+     in_dead       - result of the functions for arguments out of their domains. *)
+  Inductive interm_dec k : Set :=
+  | in_red  : redex k -> interm_dec k
+  | in_term : term -> elem_context -> interm_dec k
+  | in_val  : value k -> interm_dec k
+  | in_dead : interm_dec k.
+  Arguments in_red {k} _.    Arguments in_val {k} _.
+  Arguments in_term {k} _ _. Arguments in_dead {k}.
+
+
+  (* dec_term t k       - one step of decomposition of t from the symbol k if we
+                          have no information about subterms of t. 
+                          Domain:  term * { k : ckind | k is not dead }  
+     dec_context ec k v - one step of decomposition of a term ec[t] with an additional
+                          piece of information saying that t is a value v. 
+                          Domain:  elem_context * { (k, v) | k+>ec is not dead and
+                                                             v : value (k+>ec)     }  *)
   Parameter dec_term    : term -> forall k, interm_dec k.
   Parameter dec_context : forall ec k, value (k+>ec) -> interm_dec k.
 
@@ -136,7 +239,7 @@ Module Type RED_REF_LANG.
       end.
 
   Axiom dec_term_from_dead : 
-      forall t k, dead_ckind k -> dec_term t k = in_dead k.
+      forall t k, dead_ckind k -> dec_term t k = in_dead.
 
   Axiom dec_term_next_alive : 
       forall t k {t0 ec0}, dec_term t k = in_term t0 ec0 -> ~ dead_ckind (k+>ec0).
@@ -151,8 +254,25 @@ Module Type RED_REF_LANG.
       end.
 
   Axiom dec_context_from_dead : 
-      forall ec k (v : value (k+>ec)), 
-          dead_ckind (k+>ec) -> dec_context ec k v = in_dead k.
+      forall ec k (v : value (k+>ec)), dead_ckind (k+>ec) -> dec_context ec k v = in_dead.
+
+  Axiom dec_context_next_alive : 
+      forall ec k v {t0 ec0}, dec_context ec k v = in_term t0 ec0 -> ~ dead_ckind (k+>ec0).
+
+End DEC_STEP.
+
+
+
+Module Type RED_REF_LANG.
+
+  Declare Module R   : RED_LANG.
+  Declare Module DEC : DEC_STEP R.
+  Export R.
+  Export DEC.
+
+
+  (* Additional requirement on redexes: *)
+  Axiom redex_trivial : forall {k} (r : redex k), only_trivial r k.
 
 
   Inductive subterm_one_step : term -> term -> Prop :=
@@ -176,28 +296,31 @@ Module Type RED_REF_LANG.
       k, t |~ ec0 << ec1 -> k, t |~ ec1 << ec2 -> k,t |~ ec0 << ec2.
 
   Axiom ec_order_comp_if : forall t ec0 ec1,
-      strict_ec ec0 t -> strict_ec ec1 t -> 
+      immediate_ec ec0 t -> immediate_ec ec1 t -> 
       forall k, ~ dead_ckind (k+>ec0) -> ~ dead_ckind (k+>ec1) ->
           k, t |~ ec0 << ec1  \/  k, t |~ ec1 << ec0  \/  ec0 = ec1.
 
   Axiom ec_order_comp_fi : forall k t ec0 ec1,
-      k, t |~ ec0 << ec1  ->  strict_ec ec0 t /\ strict_ec ec1 t /\ 
+      k, t |~ ec0 << ec1  ->  immediate_ec ec0 t /\ immediate_ec ec1 t /\ 
                                   ~ dead_ckind (k+>ec0) /\ ~ dead_ckind (k+>ec1).
 
 
-  Axiom dec_term_red_empty : forall t k {r}, dec_term t k = in_red r -> only_empty t k.
-  Axiom dec_term_val_empty : forall t k {v}, dec_term t k = in_val v -> only_empty t k.
+  Axiom dec_term_red_empty : 
+      forall t k {r : redex k}, dec_term t k = in_red r -> only_empty t k.
+
+  Axiom dec_term_val_empty : 
+      forall t k {v : value k}, dec_term t k = in_val v -> only_empty t k.
 
   Axiom dec_term_term_top : 
       forall t k {t' ec}, dec_term t k = in_term t' ec -> 
           forall ec',  ~ k, t |~ ec << ec'.
 
   Axiom dec_context_red_bot : 
-      forall k ec v {r}, dec_context ec k v = in_red r -> 
+      forall k ec v {r : redex k}, dec_context ec k v = in_red r -> 
           forall ec',  ~ k, ec:[v] |~ ec' << ec.
 
   Axiom dec_context_val_bot : 
-      forall k ec v {v'}, dec_context ec k v = in_val v' -> 
+      forall k ec v {v' : value k}, dec_context ec k v = in_val v' -> 
           forall ec',  ~ k, ec:[v] |~ ec' << ec.
 
   Axiom dec_context_term_next : 
@@ -213,6 +336,9 @@ Module Type RED_REF_LANG.
 
 End RED_REF_LANG.
 
+
+
+Module RED_REF_LANG_Help.
 
   Ltac prove_st_wf := 
       intro t; constructor; induction t; 
@@ -231,14 +357,17 @@ End RED_REF_LANG.
           destruct ec; inversion H; dep_subst; clear H
       ).
 
+End RED_REF_LANG_Help.
+
+
 
 Module Type ABSTRACT_MACHINE.
 
-  Parameters term configuration : Set.
-  Parameter value : Set.
-  Parameter c_init : term -> configuration.
+  Parameters term configuration value : Set.
+  Parameter c_init  : term -> configuration.
   Parameter c_final : value -> configuration.
   Parameter transition : configuration -> configuration -> Prop.
+
 
   Inductive trans_close : configuration -> configuration -> Prop :=
   | one_step   : forall (c0 c1 : configuration), 
@@ -252,14 +381,16 @@ Module Type ABSTRACT_MACHINE.
 End ABSTRACT_MACHINE.
 
 
-Module Type SOS_SEM.
+
+(*Module Type SOS_SEM.
 
   Parameters term value : Set.
   Parameter step : term -> term -> Prop.
   Parameter value_to_term : value -> term.
 
+
   Inductive step_close : term -> value -> Prop :=
   | s_val  : forall v, step_close (value_to_term v) v
   | s_step : forall t t0 v, step t t0 -> step_close t0 v -> step_close t v.
 
-End SOS_SEM.
+End SOS_SEM.*)
