Util.v
@@ -1,134 +1,105 @@
 Require Export Wellfounded.Transitive_Closure.
-Require Export Relations.
+Require Export Relations. 
 Require Export Relation_Operators.
-Require Export List.
-Require Import Setoid.
 Require Import Program.
 Require Import Eqdep.
 
-Ltac isda := intros; simpl in *; try discriminate; auto.
 
+
+(* Transitive closures *)
 
 Section tcl.
 
-Variable A : Type.
-Variable R : relation A.
+  Variable A : Type.
+  Variable R : relation A.
 
-Notation trans_clos := (clos_trans A R).
-Notation trans_clos_l := (clos_trans_1n A R).
-Notation trans_clos_r := (clos_trans_n1 A R).
+  Notation trans_clos := (clos_trans A R).
+  Notation trans_clos_l := (clos_trans_1n A R).
+  Notation trans_clos_r := (clos_trans_n1 A R).
 
-Lemma exl : forall x y, trans_clos x y -> R x y \/ exists z, R x z /\ trans_clos z y.
-Proof with auto.
-  induction 1.
-  left...
-  right; clear IHclos_trans2; destruct IHclos_trans1 as [H1 | [u [H1 H2]]].
-  exists y...
-  exists u; split; [ assumption | econstructor 2; eauto].
-Qed.
+  Lemma exl : forall x y, trans_clos x y -> R x y \/ exists z, R x z /\ trans_clos z y.
+  Proof with auto.
+    induction 1.
+    left...
+    right; clear IHclos_trans2; destruct IHclos_trans1 as [H1 | [u [H1 H2]]].
+    exists y...
+    exists u; split; [ assumption | econstructor 2; eauto].
+  Qed.
 
-Lemma exr : forall x y, trans_clos x y -> R x y \/ exists z, R z y /\ trans_clos x z.
-Proof with auto.
-  induction 1.
-  left...
-  right; clear IHclos_trans1; destruct IHclos_trans2 as [H1 | [u [H1 H2]]].
-  exists y...
-  exists u; split; [ assumption | econstructor 2; eauto].
-Qed.
+  Lemma exr : forall x y, trans_clos x y -> R x y \/ exists z, R z y /\ trans_clos x z.
+  Proof with auto.
+    induction 1.
+    left...
+    right; clear IHclos_trans1; destruct IHclos_trans2 as [H1 | [u [H1 H2]]].
+    exists y...
+    exists u; split; [ assumption | econstructor 2; eauto].
+  Qed.
 
-Lemma tcl_l_h : forall x y z, trans_clos x y -> trans_clos_l y z -> trans_clos_l x z.
-Proof with eauto.
-  induction 1; intros...
-  econstructor 2...
-Qed.
+  Lemma tcl_l_h : forall x y z, trans_clos x y -> trans_clos_l y z -> trans_clos_l x z.
+  Proof with eauto.
+    induction 1; intros...
+    econstructor 2...
+  Qed.
 
-Lemma tcl_l : forall x y, trans_clos x y <-> trans_clos_l x y.
-Proof with eauto.
-  split; induction 1; intros...
-  constructor...
-  eapply tcl_l_h...
-  constructor...
-  econstructor 2...
-  constructor...
-Qed.
+  Lemma tcl_l : forall x y, trans_clos x y <-> trans_clos_l x y.
+  Proof with eauto.
+    split; induction 1; intros...
+    constructor...
+    eapply tcl_l_h...
+    constructor...
+    econstructor 2...
+    constructor...
+  Qed.
 
-Lemma tcl_r_h : forall x y z, trans_clos y z -> trans_clos_r x y -> trans_clos_r x z.
-Proof with eauto.
-  induction 1; intros...
-  econstructor 2...
-Qed.
+  Lemma tcl_r_h : forall x y z, trans_clos y z -> trans_clos_r x y -> trans_clos_r x z.
+  Proof with eauto.
+    induction 1; intros...
+    econstructor 2...
+  Qed.
 
-Lemma tcl_r : forall x y, trans_clos x y <-> trans_clos_r x y.
-Proof with eauto.
-  split; induction 1; intros.
-  constructor...
-  eapply tcl_r_h...
-  constructor...
-  econstructor 2...
-  constructor...
-Qed.
+  Lemma tcl_r : forall x y, trans_clos x y <-> trans_clos_r x y.
+  Proof with eauto.
+    split; induction 1; intros.
+    constructor...
+    eapply tcl_r_h...
+    constructor...
+    econstructor 2...
+    constructor...
+  Qed.
 
-Lemma Acc_tcl_l : forall x, Acc trans_clos x -> Acc trans_clos_l x.
-Proof with auto.
-  induction 1.
-  constructor; intros.
-  apply H0; rewrite tcl_l...
-Qed.
+  Lemma Acc_tcl_l : forall x, Acc trans_clos x -> Acc trans_clos_l x.
+  Proof with auto.
+    induction 1.
+    constructor; intros.
+    apply H0; rewrite tcl_l...
+  Qed.
 
-Theorem wf_clos_trans_l : well_founded R -> well_founded trans_clos_l.
-Proof with auto.
-  intros H a; apply Acc_tcl_l; apply wf_clos_trans...
-Qed.
+  Theorem wf_clos_trans_l : well_founded R -> well_founded trans_clos_l.
+  Proof with auto.
+    intros H a; apply Acc_tcl_l; apply wf_clos_trans...
+  Qed.
 
-Lemma Acc_tcl_r : forall x, Acc trans_clos x -> Acc trans_clos_r x.
-Proof with auto.
-  induction 1.
-  constructor; intros.
-  apply H0; rewrite tcl_r...
-Qed.
+  Lemma Acc_tcl_r : forall x, Acc trans_clos x -> Acc trans_clos_r x.
+  Proof with auto.
+    induction 1.
+    constructor; intros.
+    apply H0; rewrite tcl_r...
+  Qed.
 
-Theorem wf_clos_trans_r : well_founded R -> well_founded trans_clos_r.
-Proof with auto.
-  intros H a; apply Acc_tcl_r; apply wf_clos_trans...
-Qed.
+  Theorem wf_clos_trans_r : well_founded R -> well_founded trans_clos_r.
+  Proof with auto.
+    intros H a; apply Acc_tcl_r; apply wf_clos_trans...
+  Qed.
 
 End tcl.
 
 
-(*Definition opt_to_list {T} (o : option T) : list T :=
-  match o with
-  | None => nil
-  | Some x => x :: nil
-  end.*)
 
 
-Section map_injective.
+(* Some tactics *)
 
-  Variables A B : Set.
-  Variable f : A -> B.
-  Hypothesis f_injective : forall a a0 : A, f a = f a0 -> a = a0.
-
-  Lemma map_injective : forall l l0, map f l = map f l0 -> l = l0.
-  Proof.
-    induction l; destruct l0; intro H; inversion H; f_equal; auto.
-  Qed.
-
-End map_injective.
-
-
-Section streams.
-
-  Variable A : Set.
-
-  CoInductive stream :=
-  | s_nil : stream
-  | s_cons : A -> stream -> stream.
-
-  CoInductive bisim_stream : stream -> stream -> Prop :=
-  | b_nil : bisim_stream s_nil s_nil
-  | b_cons : forall (x : A) (s0 s1 : stream), bisim_stream s0 s1 -> bisim_stream (s_cons x s0) (s_cons x s1).
-
-End streams.
+Ltac clean_eqs := repeat 
+                  match goal with [H : ?x = ?x |- _] => clear H end.
 
 
 Ltac join H L R := first [ assert (H := conj L R); clear L R
@@ -137,37 +108,18 @@ Ltac join H L R := first [ assert (H := conj L R); clear L R
                          | idtac ].
 
 
-Ltac clean_eqs := repeat match goal with H : ?x = ?x |- _ => clear H end.
+Ltac dependent_destruction2 H := let i := fresh in 
+                                 remember H as i in *;
+                                 dependent destruction i;
+                                 try subst H;
+                                 clean_eqs.
 
 
-Ltac dependent_destruction2 H :=
-    let i := fresh in 
-    remember H as i in *;
-    dependent destruction i;
-    try subst H;
-    clean_eqs. 
 
 
-Ltac rec_subst H := 
-    let rec aux H R := match type of H with
-    | _ /\ _   => let G1 := fresh in let G2 := fresh in
-                  destruct H as (G1,G2); aux G1 R; aux G2 R; join H G1 G2
-    | ?x  =  _ => subst x; clear R; set (R := true)
-    | _   = ?y => subst y; clear R; set (R := true)
-    | ?x ~= ?y => try (let H' := fresh in assert (H' := H); dependent destruction H';
-                       match goal with 
-                       | _ : x ~= y |- _ => fail 2 
-                       | _               => clear H R; set (R := true) 
-                       end)
-    | _        => idtac
-    end
-    in
-    let R := fresh in
-        repeat (set (R := false);
-                aux H R; 
-                match R with false => clear R; fail | _ => clear R end).
+(* Dependent equality *)
 
-
+(* Copy of JMeq_eq_dep in Type universes *)
 Definition JMeq_eq_depT := 
     fun (U : Type) (P : U -> Type) (p q : U) (x : P p) (y : P q) (H : p = q)
         (H0 : x ~= y) =>
@@ -182,8 +134,36 @@ Definition JMeq_eq_depT :=
     end y H0.
 
 
+Ltac rec_subst H := 
+    (* H - proccesed hypothesis
+       R - helper variable that stores information if there was 
+           any substitution performed in the last aux run *)
+    let rec aux H R :=
+        match type of H with
+        | _ /\ _   => let G1 := fresh in let G2 := fresh in
+                      destruct H as (G1, G2); aux G1 R; aux G2 R; join H G1 G2
+        | ?x  =  _ => subst x; clear R; set (R := true)
+        | _   = ?y => subst y; clear R; set (R := true)
+        | ?x ~= ?y => try (dependent_destruction2 H;
+                           match goal with
+                           | _ : x ~= y |- _ => fail 2 
+                           | _               => clear R; set (R := true) 
+                           end)
+        | _        => idtac
+        end
+    in
+    let R := fresh in 
+    repeat
+    (
+        set (R := false);
+        aux H R; 
+        match R with false => clear R; fail | _ => clear R end
+    ).
+
+
 Ltac dep_subst :=
     repeat
+    (
         subst;
         match goal with 
         | G : existT _ _ _ = existT _ _ _ |- _ => dependent_destruction2 G
@@ -192,7 +172,8 @@ Ltac dep_subst :=
                                                   constr_eq tx ty;
                                                   dependent_destruction2 G
         | _ => idtac
-        end.
+        end
+    ).
 
 
 Ltac discriminateJM H := 
@@ -202,9 +183,3 @@ Ltac discriminateJM H :=
     [ apply JMeq_eq_depT; auto | discriminate (eq_dep_eq_sigT _ _ _ _ _ _ H) ]
     end.
 
-
-Implicit Arguments s_nil [A].
-Implicit Arguments s_cons [A].
-Implicit Arguments bisim_stream [A].
-Implicit Arguments b_nil [A].
-Implicit Arguments b_cons [A x s0 s1].
